code/aes/Hacl.AES_128.CTR32.NI.fst
@@ -29,13 +29,17 @@ GCM, it uses AES-128 cipher for data confidentiality.
 
 AES-CTR32 always uses the forward version of AES cipher.
 
+Note this API does not initiate or keep track of counter state, the user is supposed
+to maintain the state of counter and pass it as parameter to Encrypt/Decrypt functions.
+
 *******************************************************************************/
 
 /************************/
 /* AES-CTR32-128 API */
 /************************/\n";
 Comment
-"Allocate a buffer on stack for AES-128 key expansion and nonce"]
+"Allocate 192-byte buffer of zeros on stack for AES-128 key expansion (176-byte)
+  and nonce (16-byte)"]
 inline_for_extraction noextract
 val context_alloca: unit ->
   StackInline aes_ctx
@@ -47,7 +51,8 @@ val context_alloca: unit ->
 inline_for_extraction noextract
 let context_alloca () = create_ctx MAES Spec.AES128
 
-[@@ Comment "Allocate AES-128 context buffer using malloc for key expansion and nonce"]
+[@@ Comment "Allocate AES-128 context buffer of zeros (192-byte) using malloc
+  for key expansion and nonce"]
 inline_for_extraction
 val context_malloc:
     r:rid
@@ -59,7 +64,9 @@ val context_malloc:
     M.(modifies loc_none h0 h1) /\
     B.fresh_loc (loc_addr_of_buffer s) h0 h1 /\
     (M.loc_includes (M.loc_region_only true r) (loc_addr_of_buffer s)) /\
-    freeable s))
+    freeable s /\
+    as_seq #MUT #(stelem MAES) #(ctxlen MAES Spec.AES128) h1 s ==
+      Seq.create (size_v (ctxlen MAES Spec.AES128)) (elem_zero MAES)))
 
 let context_malloc r =
   assert (v (ctxlen MAES Spec.AES128) == 12);
@@ -68,17 +75,24 @@ let context_malloc r =
 [@@ Comment "Free AES-128 context buffer"]
 inline_for_extraction
 val context_free:
-    s:buffer (stelem MAES) { length s = v (ctxlen MAES Spec.AES128) }
+    ctx:buffer (stelem MAES) { length ctx = v (ctxlen MAES Spec.AES128) }
   -> ST.ST unit
   (requires fun h0 ->
-    freeable s /\ live h0 s)
+    freeable ctx /\ live h0 ctx)
   (ensures fun h0 _ h1 ->
-    M.modifies (loc_addr_of_buffer s) h0 h1)
+    M.modifies (loc_addr_of_buffer ctx) h0 h1)
 
-let context_free s =
-  B.free s
+let context_free ctx =
+  B.free ctx
 
-[@@ Comment "Initiate AES-128 context buffer with key expansion and nonce"]
+[@@ Comment "Initiate AES-128 context buffer with key expansion and nonce
+
+  Pads the expanded nonce buffer with zeros and copy it in little-endian
+  order to the first 16-byte of context buffer.
+  
+  Expands AES-128 key (AES key schedule) and put it in AES-128 context.
+  
+  This function is supposed to be called before using Encrypt/Decrypt functions"]
 val init:
     ctx: aes_ctx
   -> key: skey
@@ -95,7 +109,10 @@ val init:
 let init ctx key nonce = aes128_ni_init ctx key nonce
 
 
-[@@ Comment "Set nonce in AES-128 context buffer"]
+[@@ Comment "Pads the expanded nonce buffer with zeros and copy it in little-endian
+  order to the first 16-byte of AES context buffer.
+  
+  `nonce` is 12-byte buffer."]
 val set_nonce:
     ctx: aes_ctx
   -> nonce: lbuffer uint8 12ul ->
@@ -112,6 +129,8 @@ let set_nonce ctx nonce = aes_set_nonce ctx nonce
 [@@ Comment "Process 4-blocks (128-bit for each) in AES-CTR32 mode.
 
   Given that `ctx` is initiated with AES-128 key and nonce, and
+
+  `out` and `inp` are 64-byte buffers each.
   
   `counter` is the current value of counter state."]
 inline_for_extraction noextract
@@ -128,18 +147,18 @@ val update4:
       (get_nonce_s MAES Spec.AES128 h0 ctx)
       counter (as_seq h0 inp)))
 
-let update4 out inp ctx ctr = aes_update4 out inp ctx ctr
+let update4 out inp ctx counter = aes_update4 out inp ctx counter
 
 [@@ Comment "Process number of bytes in AES-CTR32 mode.
 
   Given that `ctx` is initiated with AES-128 key and nonce, and
   
-  `counter` is the initial value of counter state."]
+  `counter` is the value of counter state."]
 inline_for_extraction noextract
 val ctr:
-  len: size_t
-  -> out: lbuffer uint8 len
-  -> inp: lbuffer uint8 len
+  length_byte: size_t
+  -> out: lbuffer uint8 length_byte
+  -> inp: lbuffer uint8 length_byte
   -> ctx: aes_ctx
   -> counter: uint32
   -> ST unit
@@ -151,50 +170,58 @@ val ctr:
       (get_nonce_s MAES Spec.AES128 h0 ctx)
       counter (as_seq h0 inp)))
 
-let ctr len out inp ctx c = aes_ctr #MAES #Spec.AES128 len out inp ctx c
+let ctr length_byte out inp ctx counter = aes_ctr #MAES #Spec.AES128 length_byte out inp ctx counter
 
 
 [@@ Comment "Initiate AES-CTR32-128 context with key and nonce, and
 
   encrypt number of bytes in AES-CTR32 mode.
+
+  `key` is 16-byte buffer.
   
-  `counter` is the initial value of counter state."]
+  `nonce` is 12-byte buffer.
+  
+  `counter` is the value of counter state."]
 val ctr_encrypt:
-    len: size_t
-  -> out: lbuffer uint8 len
-  -> inp: lbuffer uint8 len
-  -> k:skey
-  -> n:lbuffer uint8 12ul
+    length_byte: size_t
+  -> out: lbuffer uint8 length_byte
+  -> inp: lbuffer uint8 length_byte
+  -> key:skey
+  -> nonce:lbuffer uint8 12ul
   -> counter:uint32
   -> ST unit
-  (requires (fun h -> live h out /\ live h inp /\ live h k /\ live h n /\
+  (requires (fun h -> live h out /\ live h inp /\ live h key /\ live h nonce /\
     disjoint out inp))
   (ensures (fun h0 _ h1 -> modifies (loc out) h0 h1 /\
     as_seq h1 out == Spec.aes_ctr32_encrypt_bytes_LE Spec.AES128
-    (as_seq h0 k) (as_seq h0 n) counter (as_seq h0 inp)))
+    (as_seq h0 key) (as_seq h0 nonce) counter (as_seq h0 inp)))
 
-let ctr_encrypt len out inp k n c = aes_ctr_encrypt #MAES #Spec.AES128 len out inp k n c
+let ctr_encrypt length_byte out inp key nonce counter = aes_ctr_encrypt #MAES #Spec.AES128 length_byte out inp key nonce counter
 
 
 [@@ Comment "Initiate AES-CTR32-128 context with key and nonce, and
 
   decrypt number of bytes in AES-CTR32 mode.
+
+  `key` is 16-byte buffer.
+  
+  `nonce` is 12-byte buffer.
   
   `counter` is the initial value of counter state.
   
   Decryption uses the forward version of AES cipher"]
 val ctr_decrypt:
-    len: size_t
-  -> out: lbuffer uint8 len
-  -> inp: lbuffer uint8 len
-  -> k:skey
-  -> n:lbuffer uint8 12ul
+    length_byte: size_t
+  -> out: lbuffer uint8 length_byte
+  -> inp: lbuffer uint8 length_byte
+  -> key:skey
+  -> nonce:lbuffer uint8 12ul
   -> counter:uint32
   -> ST unit
-  (requires (fun h -> live h out /\ live h inp /\ live h k /\ live h n /\
+  (requires (fun h -> live h out /\ live h inp /\ live h key /\ live h nonce /\
     disjoint out inp))
   (ensures (fun h0 _ h1 -> modifies (loc out) h0 h1 /\
     as_seq h1 out == Spec.aes_ctr32_decrypt_bytes_LE Spec.AES128
-    (as_seq h0 k) (as_seq h0 n) counter (as_seq h0 inp)))
-let ctr_decrypt len out inp k n c = aes_ctr_decrypt #MAES #Spec.AES128 len out inp k n c
+    (as_seq h0 key) (as_seq h0 nonce) counter (as_seq h0 inp)))
+let ctr_decrypt length_byte out inp key nonce counter = aes_ctr_decrypt #MAES #Spec.AES128 length_byte out inp key nonce counter
 
